experiments in generics; thanks to Jay

module-understanding.dfy
@@ -1,30 +1,60 @@
-//abstract module ImmutableSet {
-//    method New<V>() returns (tree: Node)
-//        requires Valid(tree)
-//        ensures Contents(tree) == multiset{}
-//
-//    method Insert(tree:Node, value:Value) returns (updated: Node)
-//        requires Valid(tree)
-//        ensures Valid(updated)
-//        ensures Contents(updated) == Contents(tree) + multiset{value};
-//
-//    method Contains(tree: Node, value: Value) returns (present: bool)
-//        requires Valid(tree)
-//        ensures present == (value in Contents(tree))
-//}
+module Comparator {
+    datatype Comparison = Less | Equal | Greater
+    datatype Comparator<!V> = Comparator(cmp:(V, V)->Comparison)
 
-abstract module Comparator {
-    predicate method lt<V>(a: V, b:V)
+    predicate IsValidComparator<V(!new)>(c:Comparator<V>)
+    {
+        // Reflexivity
+        && (forall x :: c.cmp(x, x).Equal?)
+        // Assymetry
+        && (forall x, y :: !c.cmp(x, y).Less? ==> !c.cmp(y, x).Greater?)
+        // Transitivity
+        && (forall x, y, z :: c.cmp(x, y).Less? && c.cmp(y, z).Less? ==> c.cmp(x, z).Less?)
+        // Equality
+        && (forall x, y, z :: c.cmp(x, y).Less? && c.cmp(y, z).Equal? ==> c.cmp(x, z).Less?)
+        && (forall x, y, z :: c.cmp(x, y).Equal? && c.cmp(y, z).Less? ==> c.cmp(x, z).Less?)
+    }
+    
+    function method IntComparator() : Comparator<int>
+    {
+        Comparator((a, b) =>
+            if a<b then Less else if a==b then Equal else Greater)
+    }
 
-    predicate method lte<V>(a: V, b: V)
+    function method CompareStrings(a:string, b:string) : Comparison
+    {
+        if |a| == 0 then
+            (if |b| == 0 then Equal else Less)
+        else
+            if |b| == 0 then
+               Greater 
+            else
+                if a[0] == b[0]
+                then
+                    Equal
+                else
+                    if a[0] < b[0] then Less else Greater
+    }
+
+    function method StringComparator() : Comparator<string>
+    {
+        Comparator((a, b) => CompareStrings(a, b))
+    }
+
+    lemma lemma_ComparatorsValid()
+        ensures IsValidComparator(IntComparator())
+        ensures IsValidComparator(StringComparator())
+    {
+    }
+
 }
 
-abstract module Seq {
-    import C : Comparator
-    datatype S<V> = S(contents: seq<V>)
+module Seq {
+    import opened C : Comparator
+    datatype S<!V> = S(cmp:Comparator<V>, contents: seq<V>)
 
     predicate Valid(s: S) {
-        true
+        IsValidComparator(s.cmp)
     }
 
     function Contents<V>(s: S) : multiset<V>
@@ -33,11 +63,12 @@ abstract module Seq {
         multiset(s.contents)
     }
 
-    method BaseNew<V>() returns (s: S)
+    method New<V>(cmp:Comparator<V>) returns (s: S)
+        requires IsValidComparator(cmp);
         ensures Valid(s)
         ensures Contents(s) == multiset{}
     {
-        return S([]);
+        return S(cmp, []);
     }
 
     method Insert<V>(s:S, value:V) returns (updated: S)
@@ -45,7 +76,7 @@ abstract module Seq {
         ensures Valid(updated)
         ensures Contents(updated) == Contents(s) + multiset{value};
     {
-        return S(s.contents + [value]);
+        return S(s.cmp, s.contents + [value]);
     }
 
     method Contains<V(==)>(s: S, value: V) returns (present: bool)
@@ -58,71 +89,59 @@ abstract module Seq {
     method Biggest<V>(s:S) returns (biggest: V)
         requires Valid(s)
         requires Contents(s) != multiset{}
-        ensures forall x :: x in Contents(s) ==> C.lte(x, biggest)
+        ensures forall x :: x in Contents(s) ==> !s.cmp.cmp(x, biggest).Greater?
     {
+        var cmp := s.cmp.cmp;
         biggest := s.contents[0];
         var i := 1;
         while (i < |s.contents|)
-            invariant forall x :: x in multiset(s.contents[i..i])
-                ==> C.lte(x, biggest);
+            invariant i <= |s.contents|;
+            invariant forall x :: x in s.contents[..i]
+                ==> !cmp(x, biggest).Greater?;
         {
-            if (C.lt(biggest, s.contents[i])) {
+            if (cmp(biggest, s.contents[i]).Less?) {
                 biggest := s.contents[i];
             }
+            ghost var j := i + 1;
+            i := i + 1;
         }
     }
-}
 
-module IntComparator refines Comparator {
-    predicate method lt<V>(a: int, b:int) {
-        a < b
-    }
-
-    predicate method lte(a: int, b: int) {
-        a <= b
-    }
-}
-
-module IntSeq refines Seq {
-    import C = IntComparator 
-    method New() returns (s: S<int>)
+    // Pleasant public constructors.
+    method NewIntSeq() returns (s: S<int>)
+        ensures Valid(s);
     {
-        s := BaseNew<int>();
-    }
-}
-
-module StrComparator refines Comparator {
-    predicate method lt(a: string, b:string) {
-        a < b
+        lemma_ComparatorsValid();
+        s := New(IntComparator());
     }
 
-    predicate method lte(a: string, b: string) {
-        a <= b
-    }
-}
-
-module StrSeq refines Seq {
-    import C = StrComparator 
-    method New() returns (s: S<string>)
+    method NewStringSeq() returns (s: S<string>)
+        ensures Valid(s);
     {
-        s := BaseNew<string>();
+        lemma_ComparatorsValid();
+        s := New(StringComparator());
     }
 }
 
 method Main() {
-    var intSeq := IntSeq.New();
-    intSeq := IntSeq.Insert(intSeq, 7);
-    intSeq := IntSeq.Insert(intSeq, 3);
-    intSeq := IntSeq.Insert(intSeq, 7);
-    var x1 := IntSeq.Contains(intSeq, 3);
-    var x2 := IntSeq.Contains(intSeq, 17);
-    var x3 := IntSeq.Contains(intSeq, 7);
-    print x1, x2, x3;
+    var intSeq := Seq.NewIntSeq();
+    intSeq := Seq.Insert(intSeq, 7);
+    intSeq := Seq.Insert(intSeq, 3);
+    intSeq := Seq.Insert(intSeq, 7);
+    var x1 := Seq.Contains(intSeq, 3);
+    var x2 := Seq.Contains(intSeq, 17);
+    var x3 := Seq.Contains(intSeq, 7);
+    var x4 := Seq.Biggest(intSeq);
+    print x1, " ", x2, " ", x3, " ", x4;
     print "\n";
 
-    var strSeq := StrSeq.New();
+    var strSeq := Seq.NewStringSeq();
     strSeq := Seq.Insert(strSeq, "a");
+    strSeq := Seq.Insert(strSeq, "bob");
+    strSeq := Seq.Insert(strSeq, "baby");
     strSeq := Seq.Insert(strSeq, "b");
-    var x4 := Seq.Contains(strSeq, "a");
-    print x4;
+    strSeq := Seq.Insert(strSeq, "bingo");
+    var x5 := Seq.Contains(strSeq, "a");
+    var x6 := Seq.Biggest(strSeq);
+    print x5, " ", x6, "\n";
 }
